# baseURI: http://purl.org/ub/doc/

@prefix : <http://purl.org/ub/doc/> .
@prefix dc: <http://purl.org/dc/elements/1.1/> .
@prefix owl: <http://www.w3.org/2002/07/owl#> .
@prefix rdf: <http://www.w3.org/1999/02/22-rdf-syntax-ns#> .
@prefix rdfs: <http://www.w3.org/2000/01/rdf-schema#> .
@prefix xsd: <http://www.w3.org/2001/XMLSchema#> .

:
  rdf:type owl:Ontology ;
  rdfs:label "RaCoOn documentation concepts"@en ;

.

dc:date
  rdf:type owl:AnnotationProperty ;
  rdfs:label "Date"@en ;
.
dc:description
  rdf:type owl:AnnotationProperty ;
  rdfs:label "Description"@en ;
.
dc:title
  rdf:type owl:AnnotationProperty ;
  rdfs:label "Title"@en ;
.

:AnnotationODP
  rdf:type owl:Class ;
  rdfs:comment "An ODP related to the annotation of an ontology"@en ;
  rdfs:label "Annotation ODP"@en ;
  rdfs:subClassOf :ODP ;
.
:Dialect
  rdf:type owl:Class ;
  rdfs:comment "A particular representation of the ontology's vocabulary, such that different organisations may refer to different terms in different ways"@en ;
  rdfs:label "Dialect"@en ;
  rdfs:subClassOf :MetaThing ;
.
:DocOntology
  rdf:type owl:Ontology ;
  rdfs:comment "Meta-ontology to provide ways of documenting ontologies in RDF, including design patterns and constraints"^^xsd:string ;
  owl:versionInfo "1.1.0"^^xsd:string ;
.
:EntityDescription
  rdf:type owl:Class ;
  :partofODP <http://purl.org/ub/upper/LocalNamingODP> ;
  rdfs:comment "A description of a particular entitiy to some organisation"@en ;
  rdfs:label "Entity description"@en ;
  rdfs:subClassOf :MetaThing ;
  rdfs:subClassOf [
      rdf:type owl:Restriction ;
      owl:onProperty :dialect ;
      owl:someValuesFrom :Dialect ;
    ] ;
.
:LocalNamingODP
  rdf:type :PresentationODP ;
  rdfs:comment "Design Pattern allowing ontological entities to be known by other natural language names and descriptions"^^xsd:string ;
  rdfs:comment "Design pattern for presenting organisation-specific names and terminology"@en ;
  rdfs:label "Local naming ODP"@en ;
.
:MetaThing
  rdf:type owl:Class ;
  rdfs:comment "Class of concepts that are used to meta model the ontology"@en ;
  rdfs:label "Meta thing"@en ;
  rdfs:subClassOf owl:Thing ;
.
:ODP
  rdf:type owl:Class ;
  rdfs:comment "Entities representing a particular ontology design pattern"@en ;
  rdfs:label "Ontology Design Pattern"@en ;
  rdfs:subClassOf :MetaThing ;
.
:OntologyViewAffiliation
  rdf:type owl:Class ;
  rdfs:comment "A particular view on the ontology (for an editor or viewer). Objects linked to an instance of this class through the 'parofView' property represent one view on the ontology"@en ;
  rdfs:label "Ontology view affiliation"@en ;
  rdfs:subClassOf owl:Thing ;
.
:PresentationODP
  rdf:type owl:Class ;
  rdfs:comment "An ODP related to the presentation of an ontology"@en ;
  rdfs:label "Presentation ODP"@en ;
  rdfs:subClassOf :ODP ;
.
:alsoKnownAs
  rdf:type owl:AnnotationProperty ;
  rdfs:comment "An entity that has another representation in some other form (RDF or otherwise); intentionally loose semantics"@en ;
  rdfs:domain owl:Thing ;
  rdfs:label "also known as"@en ;
  rdfs:range rdfs:Literal ;
  rdfs:subPropertyOf rdfs:comment ;
.
:dialect
  rdf:type owl:ObjectProperty ;
  rdfs:comment "Inverse of dialectOf. Describes entities that are represent dialect terms of other terms"@en ;
  rdfs:domain :EntityDescription ;
  rdfs:label "dialect"@en ;
  rdfs:range :Dialect ;
  :partofODP :LocalNamingODP ;
.
:dialectLabel
  rdf:type owl:DatatypeProperty ;
  rdfs:comment "Label to apply to an entity in a particular dialect"@en ;
  rdfs:domain :EntityDescription ;
  rdfs:label "Dialect Label"@en ;
  rdfs:range xsd:string ;
.
:dialectOf
  rdf:type owl:ObjectProperty ;
  rdfs:comment "Property to link an EntityDescription (an alternate description of an asset) with the organisation that uses that description"@en ;
  rdfs:domain :Dialect ;
  rdfs:label "Dialect Of"@en ;
  rdfs:range :EntityDescription ;
  owl:inverseOf :dialect ;
.
:dialectTerm
  rdf:type owl:ObjectProperty ;
  rdfs:comment "Represents an alternative description for a term"@en ;
  rdfs:domain owl:Thing ;
  rdfs:label "dialect term"@en ;
  rdfs:range :EntityDescription ;
  owl:inverseOf :dialectTermOf ;
.
:dialectTermOf
  rdf:type owl:ObjectProperty ;
  rdfs:comment "The term this dialect dictates"^^xsd:string ;
  rdfs:domain :EntityDescription ;
  rdfs:label "dialect term of"@en ;
  rdfs:range owl:Thing ;
.
:domainAnnotation
  rdf:type owl:AnnotationProperty ;
  rdfs:comment "A non-semantic annotation of the suggested domain of a class. Useful to imply a domain under normal circumstances, but when assertion of it in OWL may not be appropriate for reasoning or assumption reasons"@en ;
  rdfs:domain owl:Thing ;
  rdfs:label "domain annotation"@en ;
  rdfs:range owl:Thing ;
  rdfs:subPropertyOf rdfs:comment ;
.
:example
  rdf:type owl:AnnotationProperty ;
  rdfs:comment "Documents an example implmentation of a class"@en ;
  rdfs:domain owl:Thing ;
  rdfs:label "Example"@en ;
  rdfs:range rdfs:Literal ;
  rdfs:subPropertyOf rdfs:comment ;
.
:optionalConstraintAnnotation
  rdf:type owl:DatatypeProperty ;
  rdfs:comment "Annotation only (non-semantic) description of a constraint on an entity. Useful to imply formal semantics without enforcing them"@en ;
  rdfs:label "constraint annotation"@en ;
.
:partofODP
  rdf:type owl:AnnotationProperty ;
  rdfs:comment "links an entity to one or more design patterns it is part of"@en ;
  rdfs:domain owl:Thing ;
  rdfs:label "part of ODP"@en ;
  rdfs:range :ODP ;
.
:partofView
  rdf:type owl:AnnotationProperty ;
  rdfs:comment "Annotates (at a very basic level) whether this entity should be visualised as a particular view on an (OWL) ontology. Useful for when visualising the ontology itself (not its assertion data) in some OWL visualisation tool."@en ;
  rdfs:domain owl:Thing ;
  rdfs:label "partof view"@en ;
  rdfs:range owl:Thing ;
.
:rangeAnnotation
  rdf:type owl:AnnotationProperty ;
  rdfs:comment "A non-semantic annotation of the suggested domain of a class. Useful to imply a domain under normal circumstances, but when assertion of it in OWL may not be appropriate for reasoning or assumption reasons"@en ;
  rdfs:domain owl:Thing ;
  rdfs:label "range annotation"@en ;
  rdfs:range owl:Thing ;
  rdfs:subPropertyOf rdfs:comment ;
.
:turtleExample
  rdf:type owl:DatatypeProperty ;
  rdfs:comment "An example of the design pattern in use, marked up in plain text turtle"@en ;
  rdfs:comment "{@en}"^^xsd:string ;
  rdfs:domain owl:Thing ;
  rdfs:label "TTL/N3 Example"@en ;
  rdfs:range xsd:string ;
.
:version
  rdf:type owl:AnnotationProperty ;
  rdfs:comment "The version of an ontology or dataset"@en ;
  rdfs:label "version"@en ;
.

rdf:HTML
  rdfs:comment "{@en}"^^xsd:string ;
.
rdf:PlainLiteral
  rdfs:comment "{@en}"^^xsd:string ;
.
xsd:ENTITY
  rdfs:comment "{@en}"^^xsd:string ;
.
xsd:ID
  rdfs:comment "{@en}"^^xsd:string ;
.
xsd:IDREF
  rdfs:comment "{@en}"^^xsd:string ;
.
xsd:NCName
  rdfs:comment "{@en}"^^xsd:string ;
.
xsd:NMTOKEN
  rdfs:comment "{@en}"^^xsd:string ;
.
xsd:NOTATION
  rdfs:comment "{@en}"^^xsd:string ;
.
xsd:Name
  rdfs:comment "{@en}"^^xsd:string ;
.
xsd:QName
  rdfs:comment "{@en}"^^xsd:string ;
.
xsd:anySimpleType
  rdfs:comment "{@en}"^^xsd:string ;
.
xsd:anyURI
  rdfs:comment "{@en}"^^xsd:string ;
.
xsd:base64Binary
  rdfs:comment "{@en}"^^xsd:string ;
.
xsd:boolean
  rdfs:comment "{@en}"^^xsd:string ;
.
xsd:byte
  rdfs:comment "{@en}"^^xsd:string ;
.
xsd:date
  rdfs:comment "{@en}"^^xsd:string ;
.
xsd:dateTime
  rdfs:comment "{@en}"^^xsd:string ;
.
xsd:decimal
  rdfs:comment "{@en}"^^xsd:string ;
.
xsd:double
  rdfs:comment "{@en}"^^xsd:string ;
.
xsd:duration
  rdfs:comment "{@en}"^^xsd:string ;
.
xsd:float
  rdfs:comment "{@en}"^^xsd:string ;
.
xsd:gDay
  rdfs:comment "{@en}"^^xsd:string ;
.
xsd:gMonth
  rdfs:comment "{@en}"^^xsd:string ;
.
xsd:gMonthDay
  rdfs:comment "{@en}"^^xsd:string ;
.
xsd:gYear
  rdfs:comment "{@en}"^^xsd:string ;
.
xsd:gYearMonth
  rdfs:comment "{@en}"^^xsd:string ;
.
xsd:hexBinary
  rdfs:comment "{@en}"^^xsd:string ;
.
xsd:int
  rdfs:comment "{@en}"^^xsd:string ;
.
xsd:integer
  rdfs:comment "{@en}"^^xsd:string ;
.
xsd:language
  rdfs:comment "{@en}"^^xsd:string ;
.
xsd:long
  rdfs:comment "{@en}"^^xsd:string ;
.
xsd:negativeInteger
  rdfs:comment "{@en}"^^xsd:string ;
.
xsd:nonNegativeInteger
  rdfs:comment "{@en}"^^xsd:string ;
.
xsd:nonPositiveInteger
  rdfs:comment "{@en}"^^xsd:string ;
.
xsd:normalizedString
  rdfs:comment "{@en}"^^xsd:string ;
.
xsd:positiveInteger
  rdfs:comment "{@en}"^^xsd:string ;
.
xsd:short
  rdfs:comment "{@en}"^^xsd:string ;
.
xsd:string
  rdfs:comment "{@en}"^^xsd:string ;
.
xsd:time
  rdfs:comment "{@en}"^^xsd:string ;
.
xsd:token
  rdfs:comment "{@en}"^^xsd:string ;
.
xsd:unsignedByte
  rdfs:comment "{@en}"^^xsd:string ;
.
xsd:unsignedInt
  rdfs:comment "{@en}"^^xsd:string ;
.
xsd:unsignedLong
  rdfs:comment "{@en}"^^xsd:string ;
.
xsd:unsignedShort
  rdfs:comment "{@en}"^^xsd:string ;
.
