<?xml version="1.0"?>
<rdf:RDF xmlns="http://www.thalesgroup.com/rtti/PushPort/CommonTypes/v4/"
     xml:base="http://www.thalesgroup.com/rtti/PushPort/CommonTypes/v4/"
     xmlns:owl="http://www.w3.org/2002/07/owl#"
     xmlns:rdf="http://www.w3.org/1999/02/22-rdf-syntax-ns#"
     xmlns:xml="http://www.w3.org/XML/1998/namespace"
     xmlns:xsd="http://www.w3.org/2001/XMLSchema#"
     xmlns:rdfs="http://www.w3.org/2000/01/rdf-schema#">
    <owl:Ontology rdf:about="http://www.thalesgroup.com/rtti/PushPort/CommonTypes/v4"/>
    


    <!-- 
    ///////////////////////////////////////////////////////////////////////////////////////
    //
    // Datatypes
    //
    ///////////////////////////////////////////////////////////////////////////////////////
     -->

    


    <!-- http://www.thalesgroup.com/rtti/PushPort/CommonTypes/v4/ToiletStatus -->

    <rdfs:Datatype rdf:about="http://www.thalesgroup.com/rtti/PushPort/CommonTypes/v4/ToiletStatus">
        <rdfs:comment>The service status of a toilet in coach formation data.</rdfs:comment>
        <owl:equivalentClass>
            <rdfs:Datatype>
                <owl:oneOf>
                    <rdf:Description>
                        <rdf:type rdf:resource="http://www.w3.org/1999/02/22-rdf-syntax-ns#List"/>
                        <rdf:first>InService</rdf:first>
                        <rdf:rest>
                            <rdf:Description>
                                <rdf:type rdf:resource="http://www.w3.org/1999/02/22-rdf-syntax-ns#List"/>
                                <rdf:first>NotInService</rdf:first>
                                <rdf:rest>
                                    <rdf:Description>
                                        <rdf:type rdf:resource="http://www.w3.org/1999/02/22-rdf-syntax-ns#List"/>
                                        <rdf:first>Unknown</rdf:first>
                                        <rdf:rest rdf:resource="http://www.w3.org/1999/02/22-rdf-syntax-ns#nil"/>
                                    </rdf:Description>
                                </rdf:rest>
                            </rdf:Description>
                        </rdf:rest>
                    </rdf:Description>
                </owl:oneOf>
            </rdfs:Datatype>
        </owl:equivalentClass>
    </rdfs:Datatype>
    


    <!-- http://www.thalesgroup.com/rtti/PushPort/CommonTypes/v4/ToiletType -->

    <rdfs:Datatype rdf:about="http://www.thalesgroup.com/rtti/PushPort/CommonTypes/v4/ToiletType">
        <rdfs:comment>An indication of the availability of a toilet in a coach in a train formation. E.g. &quot;Unknown&quot;, &quot;None&quot; , &quot;Standard&quot; or &quot;Accessible&quot;. Note that other values may be supplied in the future without a schema change</rdfs:comment>
        <owl:equivalentClass rdf:resource="http://www.w3.org/2001/XMLSchema#string"/>
    </rdfs:Datatype>
    


    <!-- 
    ///////////////////////////////////////////////////////////////////////////////////////
    //
    // Data properties
    //
    ///////////////////////////////////////////////////////////////////////////////////////
     -->

    


    <!-- http://www.thalesgroup.com/rtti/PushPort/CommonTypes/v4/status -->

    <owl:DatatypeProperty rdf:about="http://www.thalesgroup.com/rtti/PushPort/CommonTypes/v4/status">
        <rdfs:domain rdf:resource="http://www.thalesgroup.com/rtti/PushPort/CommonTypes/v4/ToiletAvailabilityType"/>
        <rdfs:range>
            <rdfs:Datatype>
                <owl:intersectionOf rdf:parseType="Collection">
                    <rdf:Description rdf:about="http://www.thalesgroup.com/rtti/PushPort/CommonTypes/v4/ToiletStatus"/>
                    <rdf:Description rdf:about="http://www.thalesgroup.com/rtti/PushPort/CommonTypes/v4/ToiletType"/>
                </owl:intersectionOf>
            </rdfs:Datatype>
        </rdfs:range>
        <rdfs:comment>The service status of this toilet. E.g. &quot;Unknown&quot;, &quot;InService&quot; or &quot;NotInService&quot;</rdfs:comment>
    </owl:DatatypeProperty>
    


    <!-- 
    ///////////////////////////////////////////////////////////////////////////////////////
    //
    // Classes
    //
    ///////////////////////////////////////////////////////////////////////////////////////
     -->

    


    <!-- http://www.thalesgroup.com/rtti/PushPort/CommonTypes/v4/ToiletAvailabilityType -->

    <owl:Class rdf:about="http://www.thalesgroup.com/rtti/PushPort/CommonTypes/v4/ToiletAvailabilityType">
        <rdfs:comment>The availability of a toilet in coach formation data. If no availability is supplied, it should be assumed to have the value &quot;Unknown&quot;.</rdfs:comment>
    </owl:Class>
</rdf:RDF>



<!-- Generated by the OWL API (version 4.5.9.2019-02-01T07:24:44Z) https://github.com/owlcs/owlapi -->

